aarch64/Asmgenproof1.v
@@ -2044,6 +2044,7 @@ Qed.
 
 Lemma make_epilogue_correct:
   forall ge0 f m stk soff cs m' ms rs k tm,
+  (is_leaf_function f = true -> rs # (IR RA) = parent_ra cs) ->
   load_stack m (Vptr stk soff) Tptr f.(fn_link_ofs) = Some (parent_sp cs) ->
   load_stack m (Vptr stk soff) Tptr f.(fn_retaddr_ofs) = Some (parent_ra cs) ->
   Mem.free m stk 0 f.(fn_stacksize) = Some m' ->
@@ -2058,7 +2059,7 @@ Lemma make_epilogue_correct:
   /\ rs'#SP = parent_sp cs
   /\ (forall r, r <> PC -> r <> SP -> r <> RA -> r <> X16 -> rs'#r = rs#r).
 Proof.
-  intros until tm; intros LP LRA FREE AG MEXT MCS.
+  intros until tm; intros LEAF_RA LP LRA FREE AG MEXT MCS.
   exploit Mem.loadv_extends. eauto. eexact LP. auto. simpl. intros (parent' & LP' & LDP').
   exploit Mem.loadv_extends. eauto. eexact LRA. auto. simpl. intros (ra' & LRA' & LDRA').
   exploit lessdef_parent_sp; eauto. intros EQ; subst parent'; clear LDP'.
@@ -2068,6 +2069,21 @@ Proof.
   exploit (loadptr_correct XSP (fn_retaddr_ofs f)).
     instantiate (2 := rs). simpl. rewrite <- (sp_val _ _ _ AG). simpl. eexact LRA'. simpl; congruence.
   intros (rs1 & A1 & B1 & C1).
+  destruct (is_leaf_function f).
+  {
+  econstructor; econstructor; split.
+  apply exec_straight_one. simpl.
+  rewrite <- (sp_val _ _ _ AG). simpl; rewrite LP'. 
+    rewrite FREE'. eauto. auto. 
+  split. apply agree_nextinstr. apply agree_set_other; auto.
+  apply agree_change_sp with (Vptr stk soff).
+  apply agree_exten with rs; auto.
+  eapply parent_sp_def; eauto.
+  split. auto.
+  split. Simpl.
+  split. Simpl.
+  intros. Simpl.
+  }
   econstructor; econstructor; split.
   eapply exec_straight_trans. eexact A1. apply exec_straight_one. simpl. 
     simpl; rewrite (C1 SP) by auto with asmgen. rewrite <- (sp_val _ _ _ AG). simpl; rewrite LP'. 
